src/Denotational.v
@@ -1,0 +1,469 @@
+Require Import Imp.
+Require Import Maps.
+(* Require Import SfLib. for [admit] *)
+
+(* Extensional: Enumeration *)
+(* Seen this style of definition before... *)
+Definition Set' (A : Type) := list A.
+
+(* Intensional: Characteristic 'Function' *)
+Definition Bool_Set (A : Type) := A -> bool.
+
+(* Definition evens' : Bool_Set nat := evenb. *)
+
+Definition In_b {A} (a : A) (e : Bool_Set A) : Prop :=
+  e a = true.
+
+Definition Same_Set' {A} (e1 e2 : Bool_Set A) : Prop :=
+  forall x, e1 x = e2 x.
+
+(* How to define Intersection, Union, Subset ? *)
+Definition Union' {A} (e1 e2 : Bool_Set A) : Bool_Set A :=
+  fun x => orb (e1 x) (e2 x).
+
+Definition Intersection' {A} (e1 e2 : Bool_Set A)
+  : Bool_Set A :=
+  fun x => andb (e1 x) (e2 x).
+
+Definition Subset' {A} (e1 e2 : Bool_Set A) : Prop :=
+  forall x, In_b e1 x -> In_b e2 x.
+
+(* This embedding means we can always decide membership! *)
+
+  (* Let's use Prop instead! *)
+
+Definition Prop_Set (A : Type) := A -> Prop.
+
+Definition evens : Prop_Set nat :=
+  fun n => exists m, n = 2 * m.
+
+Definition In {A} (a : A) (e : Prop_Set A) : Prop :=
+  e a.
+
+Notation "x '∈' e" := (In x e) (at level 60).
+
+(*Definition odds : Prop_Set nat := ???.*)
+
+(* Membership doesn't need to be decideable! *)
+Definition terminating : Prop_Set com :=
+  fun c => forall sigma,
+      exists sigma',
+        c / sigma \\ sigma'.
+
+Lemma skip_in_terminating :
+  SKIP ∈ terminating.
+Proof.
+  unfold terminating.
+  unfold In.
+  intros.
+  exists sigma.
+  constructor.
+Qed.
+
+Definition Same_Set {A} (e1 e2 : Prop_Set A) :=
+  forall x, x ∈ e1 <-> x ∈ e2.
+
+(* How to define Intersection, Union, Subset ? *)
+Definition Union {A} (e1 e2 : Prop_Set A) : Prop_Set A := fun x => x ∈ e1 \/ x ∈ e2.
+
+Definition Intersection {A} (e1 e2 : Prop_Set A)
+  : Prop_Set A := fun x => x ∈ e1 /\ x ∈ e2.
+
+Definition Subset {A} (e1 e2 : Prop_Set A) : Prop :=
+  forall x, x ∈ e1 -> x ∈ e2.
+
+Notation "s1 ⊆ s2" := (Subset s1 s2) (at level 60).
+
+Lemma Subset_transitive {A}
+  : forall (e1 e2 e3 : Prop_Set A),
+    e1 ⊆ e2
+    -> e2 ⊆ e3
+    -> e1 ⊆ e3.
+Proof.
+  intros e1 e2 e3 ? ? x In_x.
+  apply H in In_x.
+  apply H0 in In_x.
+  apply In_x.
+Qed.
+
+Definition AExpDom := Prop_Set (nat * state).
+Definition BExpDom := Prop_Set (bool * state).
+Definition ComDom := Prop_Set (state * state).
+
+Reserved Notation "'[[' a ']]A'" (at level 40).
+Reserved Notation "'[[' b ']]B'" (at level 40).
+Reserved Notation "'[[' c ']]'" (at level 40).
+
+Fixpoint denote_A (a : aexp) : AExpDom :=
+  fun nst =>
+  match a, nst with
+  | ANum n, (n', st) =>
+    n' = n
+
+  | AId x, (n', st) =>
+    n' = st x
+
+  | APlus a1 a2, (n', st) =>
+
+    exists v1 v2,
+    (v1, st) ∈ [[ a1 ]]A
+    /\ (v2, st) ∈ [[ a2 ]]A
+    /\ n' = v1 + v2
+
+
+
+  | AMinus a1 a2, (n', st) =>
+    exists v1 v2,
+    (v1, st) ∈ [[ a1 ]]A
+    /\ (v2, st) ∈ [[ a2 ]]A
+    /\ n' = v1 - v2
+  | AMult a1 a2, (n', st) =>
+    exists v1 v2,
+    (v1, st) ∈ [[ a1 ]]A
+    /\ (v2, st) ∈ [[ a2 ]]A
+    /\ n' = v1 * v2
+  end
+where "'[[' a ']]A'" := (denote_A a).
+
+Fixpoint denote_B (b : bexp) : BExpDom :=
+  fun nst =>
+  match b, nst with
+  | BTrue, (v, st) =>
+    v = true
+  | BFalse, (v, st) =>
+    v = false
+  | BEq a1 a2, (v, st)   =>
+    exists v1 v2,
+    (v1, st) ∈ [[ a1 ]]A /\ (v2, st) ∈ [[ a2 ]]A
+    /\ (v1 = v2 -> v = true)
+    /\ (v1 <> v2 -> v = false)
+
+  | BLe a1 a2, (v, st)   =>
+    exists v1 v2,
+    (v1, st) ∈ [[ a1 ]]A /\ (v2, st) ∈ [[ a2 ]]A
+    /\ (v1 <= v2 -> v = true)
+    /\ (~ v1 <= v2 -> v = false)
+
+  | BNot b1, (v, st)     =>
+    (negb v, st) ∈ [[ b1 ]]B
+
+  | BAnd b1 b2, (v, st)  =>
+    exists v1 v2,
+    (v1, st) ∈ [[ b1 ]]B /\ (v2, st) ∈ [[ b2 ]]B
+    /\ v = (andb v1 v2)
+  end
+where "'[[' b ']]B'" := (denote_B b).
+
+
+(* Need a fixpoint operator for sets! *)
+Fail Fixpoint Fix' {A} (Gamma : Prop_Set A -> Prop_Set A) : Prop_Set A :=
+  Gamma (Fix' Gamma).
+
+Definition Fix {A} (Gamma : Prop_Set A -> Prop_Set A)
+  : Prop_Set A :=
+  fun a =>
+    forall phi, Gamma phi ⊆ phi -> a ∈ phi.
+
+Fixpoint denote_Com (c : com)
+  : ComDom :=
+  match c with
+  | SKIP =>
+    fun stst' =>
+      let (st, st') := stst' in
+      st = st'
+  | x ::= a1 =>
+    fun stst' =>
+      let (st, st') := stst' in
+      exists v,
+        (v, st) ∈ [[a1]]A
+      /\ st' = t_update st x v
+
+  | c1 ;;; c2 =>
+    fun stst' =>
+      let (st, st') := stst' in
+      exists st'',
+        (st, st'') ∈ [[c1]] /\
+      (st'', st') ∈ [[c2]]
+
+  | IFB b THEN c1 ELSE c2 FI =>
+    fun stst' =>
+      let (st, st') := stst' in
+      ((true, st) ∈ [[b]]B /\ (st, st') ∈ [[c1]])
+      \/ ((false, st) ∈ [[b]]B /\ (st, st') ∈ [[c2]])
+
+  | WHILE b DO c END =>
+      Fix (fun phi : Prop_Set _ =>
+             fun st : state * state =>
+               let (st, st') := st in
+               ((false, st) ∈ [[b]]B /\ st' = st)
+               \/ (exists st'',
+                      (true, st) ∈ [[b]]B /\
+                      (st, st'') ∈ [[c]]
+                      /\  (st'', st') ∈ phi))
+
+
+  end
+where "'[[' c ']]'" := (denote_Com c).
+
+Definition com_eq (c c' : com) : Prop :=
+  Same_Set ([[ c ]]) ([[c']]).
+
+Lemma seq_skip_opt :
+  forall c,
+    com_eq (SKIP;;; c) c.
+Proof.
+  unfold com_eq. unfold Same_Set. split; intros.
+  - destruct x; simpl in H.
+    unfold In in H.
+    destruct H as [st'' [? ?] ].
+    subst.
+    unfold In.
+    apply H0.
+  - destruct x; simpl; unfold In.
+    exists s; split.
+    reflexivity.
+    apply H.
+Qed.
+
+Lemma while_monotone :
+  forall b c (e1 e2 : Prop_Set (state * state)),
+    e1 ⊆ e2 ->
+    (fun (st : state * state) =>
+       let (st0, st') := st in
+       ((false, st0) ∈ [[b]]B /\ st' = st0) \/
+       (exists st'' : state,
+           (true, st0) ∈ [[b]]B /\ (st0, st'') ∈ [[c]] /\ (st'', st') ∈ e1))
+      ⊆
+    (fun (st : state * state) =>
+       let (st0, st') := st in
+       ((false, st0) ∈ [[b]]B /\ st' = st0) \/
+       (exists st'' : state,
+           (true, st0) ∈ [[b]]B /\ (st0, st'') ∈ [[c]] /\ (st'', st') ∈ e2)).
+Proof.
+  unfold Subset, In; intros.
+  destruct x; destruct H0 as [? | [st'' [? [? ?] ] ] ].
+  - left; eassumption.
+  - right; eexists; repeat split; try eassumption.
+    apply H; assumption.
+Qed.
+
+Lemma IF_WHILE_eq :
+  forall b c,
+    com_eq (IFB b THEN (c;;; WHILE b DO c END) ELSE SKIP FI)
+           (WHILE b DO c END).
+Proof.
+  unfold com_eq, Same_Set; split; intros.
+  - destruct x; simpl in H; unfold In in H.
+    simpl.
+    (* Need to unfold one iteration of the loop, BUT HOW? *)
+Abort.
+
+(* Restatement of the definition of Fix: if we wanted to show that *)
+(* a is in a set [phi], and we know that a is in [Fix Gamma], it  *)
+(* suffices to show that [phi] is *closed* under [Gamma]. *)
+Lemma In_Fix {A} (Gamma : Prop_Set A -> Prop_Set A) :
+  forall a,
+    a ∈ Fix Gamma
+    -> forall phi, Gamma phi ⊆ phi -> a ∈ phi.
+Proof.
+  (* By Definition. *)
+  intros; apply H; assumption.
+Qed.
+
+(* This unrolls one application of the fixpoint. *)
+Lemma Fix_Subset {A} :
+  forall Gamma
+         (Gamma_monotone :
+            forall e1 e2,
+              e1 ⊆ e2 -> Gamma e1 ⊆ Gamma e2),
+     Gamma (Fix (A := A) Gamma) ⊆ Fix Gamma.
+Proof.
+  intros Gamma ? a In_a phi Sub_Gamma.
+  (* Definition of Fix. *)
+  apply Sub_Gamma.
+  (* Monotonicity of Gamma. *)
+  eapply Gamma_monotone with (e1 := Fix Gamma); try assumption.
+  (* Definition of Fix again. *)
+  intros a' In_a'.
+  apply In_a'; assumption.
+Qed.
+
+(* We can also 're-roll' an application of the fixpoint *)
+Lemma Fix_is_Fixpoint {A} :
+  forall Gamma
+         (Gamma_monotone :
+            forall e1 e2,
+              e1 ⊆ e2 -> Gamma e1 ⊆ Gamma e2),
+    @Same_Set A (Gamma (Fix Gamma)) (Fix Gamma).
+Proof.
+  intros.
+  split; intros.
+  - apply Fix_Subset; eassumption.
+  - eapply In_Fix; try eassumption.
+    eapply Gamma_monotone.
+    apply Fix_Subset; eassumption.
+Qed.
+
+Lemma IF_WHILE_eq :
+  forall b c,
+    com_eq (IFB b THEN (c;;; WHILE b DO c END) ELSE SKIP FI)
+           (WHILE b DO c END).
+Proof.
+  unfold com_eq, Same_Set; split; intros.
+  - destruct x; simpl in H; unfold In in H.
+    simpl.
+    simpl.
+      eapply (proj1 (Fix_is_Fixpoint _ (while_monotone _ _) _));
+      unfold In in *; intros.
+    (* The denotation of [if] is built from the denotations of each branch *)
+    destruct H as [ [Denote_b [st'' [? ? ] ] ] | [Denote_b st_eq] ].
+    + right.
+      eexists; repeat split; try eassumption.
+    + left; subst; split; try eassumption; reflexivity.
+  - simpl in H.
+    (* Again, unfold one iteration of the loop. *)
+    eapply (proj2 (Fix_is_Fixpoint _ (while_monotone _ _) _)) in H.
+    (* The denotation of [while] is built from the denotation *)
+    (* of the loop body and the denotation of the terminating case. *)
+    destruct x; simpl in H; unfold In in H.
+    destruct H as [ [? ?] | [st' [Denote_b [? ?] ] ] ].
+    + simpl; unfold In.
+      right; split; subst; try eassumption; reflexivity.
+    + simpl; unfold In; left; repeat split; try eassumption.
+      eexists; repeat split; eassumption.
+Qed.
+
+Lemma Denotational_A_BigStep_Equivalent :
+  forall a st,
+    (aeval st a, st) ∈ [[a]]A.
+Proof.
+  intros;
+  induction a; simpl; try solve [constructor]; unfold In;
+  eexists _, _; repeat split; try eassumption.
+Qed.
+
+Lemma Denotational_B_BigStep_Equivalent :
+  forall b st,
+    (beval st b, st) ∈ [[b]]B.
+Proof.
+Admitted.
+
+Lemma BigStep_Denotational_Equivalent :
+  forall c st st',
+    c / st \\ st' -> (st, st') ∈ [[c]].
+Proof.
+  intros.
+  induction H; simpl; try solve [econstructor]; unfold In.
+  - (* E_Ass *)
+    eexists; split; try reflexivity.
+    rewrite <- H; eapply Denotational_A_BigStep_Equivalent.
+  - (* E_Seq *)
+    eexists; split; try reflexivity; eassumption.
+  - (* E_IfTrue *)
+    left; subst; split; try eassumption.
+    rewrite <- H; eapply Denotational_B_BigStep_Equivalent.
+  - (* E_IfFalse *)
+    right; subst; split; try eassumption.
+    rewrite <- H; eapply Denotational_B_BigStep_Equivalent.
+  - (* E_WhileEnd *)
+    apply Fix_is_Fixpoint.
+    apply while_monotone.
+    left.
+    split; try reflexivity.
+    rewrite <- H; apply Denotational_B_BigStep_Equivalent.
+  - (* E_WhileLoop *)
+    apply Fix_is_Fixpoint.
+    apply while_monotone.
+    right.
+    eexists; repeat split; try eassumption.
+    rewrite <- H; apply Denotational_B_BigStep_Equivalent.
+Qed.
+
+Lemma BigStep_A_Denotational_Equivalent :
+  forall a st v,
+    (v, st) ∈ [[a]]A
+    -> v = aeval st a.
+Proof.
+  induction a; simpl; intros st v H;
+    unfold In in H; try eassumption.
+  - destruct H as [v1 [v2 [denote_a1 [denote_a2 v_eq] ] ] ]; subst.
+    apply IHa1 in denote_a1; apply IHa2 in denote_a2.
+    subst; reflexivity.
+  - destruct H as [v1 [v2 [denote_a1 [denote_a2 v_eq] ] ] ]; subst.
+    apply IHa1 in denote_a1; apply IHa2 in denote_a2.
+    subst; reflexivity.
+  - destruct H as [v1 [v2 [denote_a1 [denote_a2 v_eq] ] ] ]; subst.
+    apply IHa1 in denote_a1; apply IHa2 in denote_a2.
+    subst; reflexivity.
+Qed.
+
+Lemma BigStep_B_Denotational_Equivalent :
+  forall b st v,
+    (v, st) ∈ [[b]]B
+    -> v = beval st b.
+Proof.
+Admitted.
+
+(* Yet another restatement of the definition of Fix; this time as *)
+(* the principle of mathematical induction. *)
+Lemma Fix_ind {A}
+      (P : A -> Prop)
+      (Gamma : Prop_Set A -> Prop_Set A)
+  : forall a,
+    (Gamma P ⊆ P)
+    -> a ∈ Fix Gamma
+    -> P a.
+Proof.
+  intros a P_Ind a_In.
+  eapply In_Fix; try eassumption.
+Qed.
+
+Lemma Denotational_BigStep_Equivalent :
+  forall c st st',
+    (st, st') ∈ [[c]] -> c / st \\ st'.
+Proof.
+  induction c; unfold In; simpl; intros st st' denote_c.
+  - (* SKIP *)
+    subst; econstructor.
+  - (* Assignment *)
+    destruct denote_c as [v [? ?] ].
+    subst; econstructor.
+    erewrite BigStep_A_Denotational_Equivalent; try reflexivity; assumption.
+  - (* Sequence *)
+    destruct denote_c as [v [denote_c1 denote_c2] ].
+    subst; econstructor.
+    + apply IHc1; eassumption.
+    + apply IHc2; eassumption.
+  - (* Conditional *)
+    destruct denote_c as [ [denote_b denote_c1] | [denote_b denote_c2] ].
+    + constructor.
+      erewrite BigStep_B_Denotational_Equivalent; try reflexivity; assumption.
+      apply IHc1; eassumption.
+    + apply E_IfFalse.
+      erewrite BigStep_B_Denotational_Equivalent; try reflexivity; assumption.
+      apply IHc2; eassumption.
+  - apply Fix_is_Fixpoint in denote_c; try apply while_monotone.
+    destruct denote_c as [ [denote_b st_eq]
+                         | [st'' [denote_b [denote_c ? ] ] ] ].
+    + rewrite st_eq; econstructor.
+      erewrite BigStep_B_Denotational_Equivalent; try reflexivity; assumption.
+    + eapply E_WhileLoop.
+      erewrite BigStep_B_Denotational_Equivalent; try reflexivity; assumption.
+      apply IHc; eassumption.
+      change st'' with (fst (st'', st')).
+      change st' with (snd (st'', st')) at 2.
+      pattern (st'', st').
+      (* Hmmmm... we're (almost) back to where we started! *)
+      (* Why can't we apply the Inductive Hypothesis? *)
+      eapply Fix_ind; try eassumption.
+      generalize IHc; clear.
+      intros IHc [st'' st']
+             [ [denote_b st_eq]
+             | [st''0 [denote_b [denote_c ? ] ] ] ].
+      * subst; econstructor.
+        erewrite BigStep_B_Denotational_Equivalent; try reflexivity; assumption.
+      * econstructor.
+        erewrite BigStep_B_Denotational_Equivalent; try reflexivity; assumption.
+        apply IHc; eassumption.
+        apply H.
+Qed.
